src/HaskCoreVars.v
@@ -6,6 +6,7 @@ Generalizable All Variables.
 Require Import Preamble.
 Require Import General.
 Require Import Coq.Strings.String.
+Require Import HaskLiteralsAndTyCons.
 
 (* GHC uses a single type for expression variables, type variables, and coercion variables; this is that type *)
 Variable CoreVar            : Type.                                               Extract Inlined Constant CoreVar    => "Var.Var".
@@ -13,3 +14,18 @@ Variable coreVar_eq         : forall (a b:CoreVar), sumbool (a=b) (not (a=b)).  
 Variable coreVarToString    : CoreVar      -> string.             Extract Inlined Constant coreVarToString => "outputableToString".
 Instance CoreVarEqDecidable : EqDecidable CoreVar := { eqd_dec  := coreVar_eq      }.
 Instance CoreVarToString    : ToString CoreVar    := { toString := coreVarToString }.
+
+Variable CoreTyCon       : Type.                      Extract Inlined Constant CoreTyCon            => "TyCon.TyCon".
+
+(* because Haskell's 3-tuples (triples) are distinct from both ((x,y),z) and (x,(y,z)), we need a new type: *)
+Inductive triple {A B C:Type} :=
+| mkTriple : A -> B -> C -> triple.
+Notation "a ** b ** c" := (mkTriple a b c) (at level 20).
+Extract Inductive triple => "(,,)" [ "(,,)" ].
+
+Inductive CoreAltCon :=
+| DataAlt : CoreDataCon -> CoreAltCon
+| LitAlt  : HaskLiteral -> CoreAltCon
+| DEFAULT :                CoreAltCon.
+Extract Inductive CoreAltCon =>
+  "CoreSyn.AltCon" [ "CoreSyn.DataAlt" "CoreSyn.LitAlt" "CoreSyn.DEFAULT" ].
