src/HaskWeakVars.v
@@ -8,7 +8,7 @@ Require Import General.
 Require Import Coq.Strings.String.
 Require Import Coq.Lists.List.
 Require Import HaskKinds.
-Require Import HaskCoreLiterals.
+Require Import HaskLiteralsAndTyCons.
 Require Import HaskCoreVars.
 Require Import HaskCoreTypes.
 Require Import HaskWeakTypes.
@@ -46,54 +46,12 @@ Variable getTyConTyVars_   : CoreTyCon   -> list CoreVar.  Extract Inlined Const
 Definition tyConTyVars (tc:CoreTyCon) :=
   General.filter (map (fun x => match coreVarToWeakVar x with WTypeVar v => Some v | _ => None end) (getTyConTyVars_ tc)).
   Opaque tyConTyVars.
-Definition tyConKind (tc:TyCon) : list Kind :=
-  map (fun (x:WeakTypeVar) => x:Kind) (tyConTyVars tc).
+Definition tyConKind (tc:TyCon) : list Kind := map (fun (x:WeakTypeVar) => x:Kind) (tyConTyVars tc).
 
 Variable rawTyFunKind : CoreTyCon -> Kind. Extract Inlined Constant rawTyFunKind => "(coreKindToKind . TyCon.tyConKind)".
 
 Definition tyFunKind (tc:TyFun) : ((list Kind) * Kind) :=
   splitKind (rawTyFunKind tc).
-
-(*
-(* EqDecidable instances for all of the above *)
-Instance WeakCoerVarEqDecidable : EqDecidable WeakCoerVar.
-  apply Build_EqDecidable.
-  intros.
-  destruct v1 as [cv1 t1a t1b].
-  destruct v2 as [cv2 t2a t2b].
-  destruct (eqd_dec cv1 cv2); subst.
-    destruct (eqd_dec t1a t2a); subst.
-    destruct (eqd_dec t1b t2b); subst.
-    left; auto.
-    right; intro; apply n; inversion H; subst; auto.
-    right; intro; apply n; inversion H; subst; auto.
-    right; intro; apply n; inversion H; subst; auto.
-    Defined.
-
-Instance WeakExprVarEqDecidable : EqDecidable WeakExprVar.
-  apply Build_EqDecidable.
-  intros.
-  destruct v1 as [cv1 k1].
-  destruct v2 as [cv2 k2].
-  destruct (eqd_dec cv1 cv2); subst.
-    destruct (eqd_dec k1 k2); subst.
-    left; auto.
-    right; intro; apply n; inversion H; subst; auto.
-    right; intro; apply n; inversion H; subst; auto.
-    Defined.
-
-Instance WeakVarEqDecidable : EqDecidable WeakVar.
-  apply Build_EqDecidable.
-  induction v1; destruct v2; try (right; intro q; inversion q; fail) ; auto;
-     destruct (eqd_dec w w0); subst.
-     left; auto.
-     right; intro X; apply n; inversion X; auto.
-     left; auto.
-     right; intro X; apply n; inversion X; auto.
-     left; auto.
-     right; intro X; apply n; inversion X; auto.
-  Defined.
-*)
 
 Instance WeakVarToString : ToString WeakVar :=
   { toString := fun x => toString (weakVarToCoreVar x) }.
